Hs/Example.lean
@@ -1,0 +1,61 @@
+import Hs.HsTerm
+import Hs.Algorithm
+import SystemFD.Algorithm
+
+def idHsTerm : HsTerm := `λ{`#0} `#0
+def idHsType : HsTerm := `∀{`★} `#0 → `#1
+
+def idTypeKinding : [] ⊢s idHsType : `★ := by
+  unfold idHsType;
+  apply HsJudgment.allt;
+  case _ => apply HsJudgment.ax (HsJudgment.wfnil)
+  case _ =>
+    apply HsJudgment.arrow;
+    case _ =>
+      apply HsJudgment.var; apply HsJudgment.wfkind; apply HsJudgment.ax (HsJudgment.wfnil);
+      apply HsJudgment.wfnil; unfold Frame.get_type; unfold dnth; unfold Frame.apply; simp;
+    case _ =>
+      apply HsJudgment.var;
+      apply HsJudgment.wfempty; apply HsJudgment.wfkind; apply HsJudgment.ax (HsJudgment.wfnil);
+      apply HsJudgment.wfnil;
+      unfold Frame.get_type; unfold dnth; unfold Frame.apply; simp; unfold Frame.apply; simp
+
+def idTyping : [] ⊢s idHsTerm : idHsType := by
+ unfold idHsTerm; unfold idHsType;
+ apply HsJudgment.implicitAllI;
+ apply HsJudgment.lam;
+   apply HsJudgment.var; apply HsJudgment.wfkind; apply HsJudgment.ax (HsJudgment.wfnil);
+   apply HsJudgment.wfnil; unfold Frame.get_type; unfold dnth; unfold Frame.apply; simp;
+   apply HsJudgment.var;
+     apply HsJudgment.wftype; apply HsJudgment.var;
+     apply HsJudgment.wfkind; apply HsJudgment.ax (HsJudgment.wfnil);
+       apply HsJudgment.wfnil;
+       unfold Frame.get_type; unfold dnth; unfold Frame.apply; simp;
+       apply HsJudgment.wfkind; apply HsJudgment.ax (HsJudgment.wfnil);
+       apply HsJudgment.wfnil;
+     unfold Frame.get_type; unfold dnth; unfold Frame.apply; simp;
+   case _ =>
+     apply HsJudgment.arrow;
+     apply HsJudgment.var;
+     apply HsJudgment.wfkind; apply HsJudgment.ax (HsJudgment.wfnil); apply HsJudgment.wfnil;
+     unfold Frame.get_type; unfold dnth; unfold Frame.apply; simp;
+     apply HsJudgment.var; apply HsJudgment.wfempty; apply HsJudgment.wfkind;
+     apply HsJudgment.ax (HsJudgment.wfnil); apply HsJudgment.wfnil;
+     unfold Frame.get_type; unfold dnth; unfold Frame.apply; simp; unfold Frame.apply; simp
+ apply HsJudgment.ax (HsJudgment.wfnil);
+ apply HsJudgment.arrow; apply HsJudgment.var;
+   apply HsJudgment.wfkind; apply HsJudgment.ax (HsJudgment.wfnil); apply HsJudgment.wfnil;
+   unfold Frame.get_type; unfold dnth; unfold Frame.apply; simp
+ apply HsJudgment.var;
+ apply HsJudgment.wfempty; apply HsJudgment.wfkind; apply HsJudgment.ax (HsJudgment.wfnil); apply HsJudgment.wfnil;
+ unfold Frame.get_type; simp; unfold Frame.apply; simp
+
+def idType := compile [] idHsType `★ idTypeKinding
+def idTerm := compile [] idHsTerm idHsType idTyping
+
+#guard idType == .some (∀[★] #0 -t> #1)
+#guard idTerm == .some (Λ[★]`λ[#0] #0)
+#guard idType == do { let t <- idTerm; infer_type [] t }
+
+#eval idType
+#eval idTerm
