Hs/Metatheory/Preservation2.lean
@@ -1,0 +1,111 @@
+import Hs.Algorithm
+
+
+inductive HsKindLike : HsTerm -> Prop where
+| HsType : HsKindLike `★
+| HsArrK : HsKindLike k -> HsKindLike k' -> HsKindLike (k `-k> k')
+
+inductive CompileCtx : Ctx HsTerm -> Ctx Term -> Prop where
+| nil : CompileCtx [] []
+| empty :
+  CompileCtx Γ Γ' ->
+  CompileCtx (.empty :: Γ) (.empty :: Γ')
+| kind :
+  CompileCtx Γ Γ' ->
+  (j1 : Γ ⊢s A : `□) ->
+  compile Γ A `□ j1 = .some A' ->
+  CompileCtx (.kind A :: Γ) (.kind A' :: Γ')
+| type :
+  CompileCtx Γ Γ' ->
+  (j1 : Γ ⊢s A : `★) ->
+  compile Γ A `★ j1 = .some A' ->
+  CompileCtx (.type A :: Γ) (.type A' :: Γ')
+| term :
+  CompileCtx Γ Γ' ->
+  (j1 : Γ ⊢s A : `★)  ->
+  (j2 : Γ ⊢s t : τ) ->
+  compile Γ A `★ j = .some A' ->
+  compile Γ t τ j2 = .some t' ->
+  CompileCtx (.term A t :: Γ) (.term A' t' :: Γ')
+
+
+theorem compile_ctx_wf :
+  ⊢s Γ ->
+  CompileCtx Γ Γ' ->
+  ⊢ Γ' := by
+intro h1 h2;
+induction h2;
+case _ => apply Judgment.wfnil
+case _ h1 ih1 =>
+  cases h1; case _ h1 =>
+  apply Judgment.wfempty;
+  apply ih1 h1;
+case _ h1 j1 cc ih =>
+ apply Judgment.wfkind;
+ sorry
+ sorry
+case _ => sorry
+case _ => sorry
+
+theorem kinding_uniqueness :
+  HsKindLike τ ->
+  Γ ⊢s τ : k ->
+  Γ ⊢s τ : k' ->
+  k = k' :=
+ by
+intro h j1 j2
+induction τ generalizing Γ k k'
+all_goals (cases h)
+case _ => sorry
+case _ ih1 ih2 kl1 kl2 =>
+  have lem1 := @ih1 Γ `□ `□ kl1;
+  sorry
+
+theorem compile_preserves_kinds :
+  HsKindLike t ->
+  τ = `□ ->
+  (j : Γ ⊢s t : τ) ->
+  compile Γ t τ j = .some t' ->
+  CompileCtx Γ Γ' ->
+  Γ' ⊢ t' : .kind := by
+ intro h e j c cc;
+ induction Γ, t, τ, j using compile.induct generalizing t'
+ all_goals try (cases e)
+ all_goals try (cases h)
+ case _ =>
+   unfold compile at c; cases c;
+   apply Judgment.ax;
+   sorry
+ case _ j1 j2 ih1 ih2 kl1 kl2 =>
+   unfold compile at c; simp at c;
+   rw[Option.bind_eq_some] at c;
+   cases c; case _ w1 c1 =>
+   cases c1; case _ c1 c2 =>
+   rw[Option.bind_eq_some] at c2;
+   cases c2; case _ w2 c2 =>
+   cases c2; case _ c2 c3 =>
+   cases c3;
+   have ih1' := @ih1 w1 kl1 rfl c1 cc;
+   have ih2' := @ih2 w2 kl2 rfl c2 cc;
+   apply Judgment.allk;
+   apply ih1';
+   apply ih2'
+-- bogus cases
+ case _ j1 ih1 =>  sorry
+ case _ => sorry
+ case _ => sorry
+ case _ => sorry
+
+
+
+def is_type : Ctx HsTerm -> HsTerm -> Option Unit
+| Γ, .HsBind2 .arrow k k' => do
+  let _ <- is_type Γ k
+  let _ <- is_type (.empty :: Γ) k'
+  .some ()
+| Γ, .HsBind2 .farrow k k' => do
+  let _ <- is_type Γ k
+  let _ <- is_type (.empty :: Γ) k'
+  .some ()
+| Γ, `#x => if (Γ d@x).is_datatype then .some () else .none
+| _, _ => .none
